Lesson 28: Another Computational Method of Solving a Linear System

Classwork

**Example 1**

Use what you noticed about adding equivalent expressions to solve the
following system by elimination:

$$\left\{ \begin{array}{r}
6x - 5y = 21 \\
2x + 5y = - 5
\end{array} \right.\ $$

**Example 2**

Solve the following system by elimination:

$$\left\{ \begin{array}{r}
 - 2x + 7y = 5 \\
4x - 2y = 14\ \ \ 
\end{array} \right.\ $$

**Example 3**

Solve the following system by elimination:

$$\left\{ \begin{array}{r}
7x - 5y = - 2 \\
3x - 3y = 7\ \ \ 
\end{array} \right.\ $$

Exercises

Each of the following systems has a solution. Determine the solution to
the system by eliminating one of the variables. Verify the solution
using the graph of the system.

$\left\{ \begin{array}{r}
6x - 7y = - 10 \\
3x + 7y = - 8\ \ \ 
\end{array} \right.\ $

$\left\{ \begin{array}{r}
x - 4y = 7\ \  \\
5x + 9y = 6
\end{array} \right.\ $

$\left\{ \begin{array}{r}
2x - 3y = - 5 \\
3x + 5y = 1\ \ \ 
\end{array} \right.\ $

Lesson Summary

Systems of linear equations can be solved by eliminating one of the
variables from the system. One way to eliminate a variable is by setting
both equations equal to the same variable and then writing the
expressions equal to one another.

Example: Solve the system $\left\{ \begin{array}{r}
y = 3x - 4 \\
y = 2x + 1
\end{array} \right.\ .$

Since the expressions $3x - 4$ and $2x + 1$ are both equal to $y,$ they
can be set equal to each other and the new equation can be solved for
$x$:

$$3x - 4 = 2x + 1$$

Another way to eliminate a variable is by multiplying each term of an
equation by the same constant to make an equivalent equation. Then, use
the equivalent equation to eliminate one of the variables and solve the
system.

Example: Solve the system $\left\{ \begin{array}{r}
2x + y = 8 \\
x + y = 10
\end{array} \right.\ .$

Multiply the second equation by $- 2$ to eliminate the $x.$

$${- 2(x + y = 10)
}{- 2x - 2y = - 20}$$

Now we have the system $\left\{ \begin{array}{r}
2x + y = 8 \\
 - 2x - 2y = - 20
\end{array} \right.\ .$

When the equations are added together, the $x$ is eliminated.

$${2x + y - 2x - 2y = 8 + ( - 20)
}{y - 2y = 8 + ( - 20)}$$

Once a solution has been found, verify the solution graphically or by
substitution.

Problem Set

Determine the solution, if it exists, for each system of linear
equations. Verify your solution on the coordinate plane.

$\left\{ \begin{array}{r}
\frac{1}{2}x + 5 = y \\
2x + y = 1
\end{array} \right.\ $

$\left\{ \begin{array}{r}
9x + 2y = 9\  \\
 - 3x + y = 2
\end{array} \right.\ $

$\left\{ \begin{array}{r}
y = 2x - 2\ \  \\
2y = 4x - 4
\end{array} \right.\ $

$\left\{ \begin{array}{r}
8x + 5y = 19 \\
 - 8x + y = - 1
\end{array} \right.\ $

$\left\{ \begin{array}{r}
x + 3 = y\ \ \ \ \  \\
3x + 4y = 7
\end{array} \right.\ $

$\left\{ \begin{array}{r}
y = 3x + 2\ \ \ \ \ \ \ \  \\
4y = 12 + 12x
\end{array} \right.\ $

$\left\{ \begin{array}{r}
4x - 3y = 16\ \ \ \  \\
 - 2x + 4y = - 2
\end{array} \right.\ $

$\left\{ \begin{array}{r}
2x + 2y = 4\ \  \\
12 - 3x = 3y
\end{array} \right.\ $

$\left\{ \begin{array}{r}
y = - 2x + 6 \\
3y = x - 3\ \ \ \ 
\end{array} \right.\ $

$\left\{ \begin{array}{r}
y = 5x - 1\ \ \ \  \\
10x = 2y + 2
\end{array} \right.\ $

$\left\{ \begin{array}{r}
3x - 5y = 17 \\
6x + 5y = 10
\end{array} \right.\ $

$\left\{ \begin{array}{r}
y = \frac{4}{3}x - 9 \\
y = x + 3\ \ \ 
\end{array} \right.\ $

$\left\{ \begin{array}{r}
4x - 7y = 11 \\
x + 2y = 10\ \ 
\end{array} \right.\ $

$\left\{ \begin{array}{r}
21x + 14y = 7 \\
12x + 8y = 16
\end{array} \right.\ $
