Lesson 2: Multiplication of Numbers in Exponential Form

Classwork

In general, if $x$ is any number and$\ m$,$\ n$ are positive integers,
then

$x^{m} \bullet x^{n} = x^{m + n}$

because

$x^{m} \times x^{n} = \underset{m\ \text{times}}{\overset{(x\cdots x)}{︸}} \times \underset{n\ \text{times}}{\overset{(x\cdots x)}{︸}} = \underset{m + n\ \text{times}}{\overset{(x\cdots x)}{︸}} = x^{m + n}\text{.}$

+----------------------------------------+-----------------------------------------------+
| Exercise 1                             | Exercise 5                                    |
|                                        |                                               |
| $$14^{23} \times 14^{8} =$$            | Let $a$ be a number.                          |
|                                        |                                               |
|                                        | $$a^{23} \bullet a^{8} =$$                    |
+========================================+===============================================+
| Exercise 2                             | Exercise 6                                    |
|                                        |                                               |
| $$( - 72)^{10} \times ( - 72)^{13} =$$ | Let $f$ be a number.                          |
|                                        |                                               |
|                                        | $$f^{10} \bullet f^{13} =$$                   |
+----------------------------------------+-----------------------------------------------+
| Exercise 3                             | Exercise 7                                    |
|                                        |                                               |
| $$5^{94} \times 5^{78} =$$             | Let $b$ be a number.                          |
|                                        |                                               |
|                                        | $$b^{94} \bullet b^{78} =$$                   |
+----------------------------------------+-----------------------------------------------+
| Exercise 4                             | Exercise 8                                    |
|                                        |                                               |
| $$( - 3)^{9} \times ( - 3)^{5} =$$     | Let $x$ be a positive integer. If             |
|                                        | $( - 3)^{9} \times ( - 3)^{x} = ( - 3)^{14}$, |
|                                        | what is $x$?                                  |
+----------------------------------------+-----------------------------------------------+

What would happen if there were more terms with the same base? Write an
equivalent expression for each problem.

+----------------------------------------+----------------------------------------------------+
| Exercise 9                             | Exercise 10                                        |
|                                        |                                                    |
| $$9^{4} \times 9^{6} \times 9^{13} =$$ | $$2^{3} \times 2^{5} \times 2^{7} \times 2^{9} =$$ |
+========================================+====================================================+

Can the following expressions be written in simpler form? If so, write
an equivalent expression. If not, explain why not.

+-------------------------------------------------------------------+-----------------------------------------------+
| Exercise 11                                                       | Exercise 14                                   |
|                                                                   |                                               |
| $$6^{5} \times 4^{9} \times 4^{3} \times 6^{14} =$$               | $$2^{4} \times 8^{2} = 2^{4} \times 2^{6} =$$ |
+===================================================================+===============================================+
| Exercise 12                                                       | Exercise 15                                   |
|                                                                   |                                               |
| $$( - 4)^{2} \bullet 17^{5} \bullet ( - 4)^{3} \bullet 17^{7} =$$ | $$3^{7} \times 9 = 3^{7} \times 3^{2} =$$     |
+-------------------------------------------------------------------+-----------------------------------------------+
| Exercise 13                                                       | Exercise 16                                   |
|                                                                   |                                               |
| $$15^{2} \bullet 7^{2} \bullet 15 \bullet 7^{4} =$$               | $5^{4}{\times 2}^{11} =$                      |
+-------------------------------------------------------------------+-----------------------------------------------+

Exercise 17

Let $x$ be a number. Rewrite the expression in a simpler form.

$$\left( 2x^{3} \right)\left( 17x^{7} \right) =$$

Exercise 18

Let $a$ and $b$ be numbers. Use the distributive law to rewrite the
expression in a simpler form.

$$a(a + b) =$$

Exercise 19

Let $a$ and $b$ be numbers. Use the distributive law to rewrite the
expression in a simpler form.

$b(a + b) =$

Exercise 20

Let $a$ and $b$ be numbers. Use the distributive law to rewrite the
expression in a simpler form.

$$(a + b)(a + b) =$$

In general, if $x$ is nonzero and$\ m,\ n\ $are positive integers, then

$$\frac{x^{m}}{x^{n}} = x^{m - n}\text{.}$$

+--------------------------------------+-----------------------------------------------------------------------------+
| Exercise 21                          | Exercise 23                                                                 |
|                                      |                                                                             |
| $$\frac{7^{9}}{7^{6}} =$$            | $$\frac{\left( \frac{8}{5} \right)^{9}}{\left( \frac{8}{5} \right)^{2}} =$$ |
+======================================+=============================================================================+
| Exercise 22                          | Exercise 24                                                                 |
|                                      |                                                                             |
| $$\frac{( - 5)^{16}}{( - 5)^{7}} =$$ | $$\frac{13^{5}}{13^{4}} =$$                                                 |
+--------------------------------------+-----------------------------------------------------------------------------+

Exercise 25

Let $a$*,* $b$ be nonzero numbers. What is the following number?

$$\frac{\left( \frac{a}{b} \right)^{9}}{\left( \frac{a}{b} \right)^{2}} =$$

Exercise 26

Let $x$ be a nonzero number. What is the following number?

$$\frac{x^{5}}{x^{4}} =$$

Can the following expressions be written in simpler forms? If yes, write
an equivalent expression for each problem. If not, explain why not.

+-------------------------------------------------+-------------------------------------------------------------------+
| Exercise 27                                     | Exercise 29                                                       |
|                                                 |                                                                   |
| $$\frac{2^{7}}{4^{2}} = \frac{2^{7}}{2^{4}} =$$ | $$\frac{3^{5} \bullet 2^{8}}{3^{2} \bullet 2^{3}} =$$             |
+=================================================+===================================================================+
| Exercise 28                                     | Exercise 30                                                       |
|                                                 |                                                                   |
| $$\frac{3^{23}}{27} = \frac{3^{23}}{3^{3}} =$$  | $$\frac{( - 2)^{7} \bullet 95^{5}}{( - 2)^{5} \bullet 95^{4}} =$$ |
+-------------------------------------------------+-------------------------------------------------------------------+

Exercise 31

Let $x$ be a number. Write each expression in a simpler form.

$\frac{5}{x^{3}}$ $\left( 3x^{8} \right) =$

$\frac{5}{x^{3}}$ $\left( - 4x^{6} \right) =$

$\frac{5}{x^{3}}$ $\left( 11x^{4} \right) =$

Exercise 32

Anne used an online calculator to multiply
$2\ 000\ 000\ 000\  \times 2\ 000\ \ 000\ \ 000\ \ 000$. The answer
showed up on the calculator as $4e + 21$, as shown below. Is the answer
on the calculator correct? How do you know?

![Macintosh HD:Users:shassan:Desktop:calc screen
shot.tiff](.\grade8lessonsmd\media/media/image1.png){width="2.470138888888889in"
height="1.4958333333333333in"}

Problem Set

1.  A certain ball is dropped from a height of $x$ feet. It always
    bounces up to $\frac{2}{3}$ $x$ feet. Suppose the ball is dropped
    from $10$ feet and is stopped exactly when it touches the ground
    after the $30$^th^ bounce. What is the total distance traveled by
    the ball? Express your answer in exponential notation.

  ------------------------------------------------------------------------
   Bounce  Computation of   Total Distance Traveled (in feet)
           Distance         
           Traveled in      
           Previous Bounce  
  -------- ---------------- ----------------------------------------------
   $$1$$                    

   $$2$$                    

   $$3$$                    

   $$4$$                    

   $$30$$                   

   $$n$$                    
  ------------------------------------------------------------------------

1.  If the same ball is dropped from $10$ feet and is caught exactly at
    the highest point after the $25$^th^ bounce, what is the total
    distance traveled by the ball? Use what you learned from the last
    problem.

2.  Let $a$ and$\ b$ be numbers and $b \neq 0$, and let $m\ $and $n$ be
    positive integers. Write each expression using the fewest number of
    bases possible:

  ----------------------------------------------------------------------------------------------------------------------------------------------------------------
  $$( - 19)^{5} \bullet ( - 19)^{11} =$$                                            $${2.7}^{5} \times {2.7}^{3} =$$
  --------------------------------------------------------------------------------- ------------------------------------------------------------------------------
  $$\frac{7^{10}}{7^{3}} =$$                                                        $$\left( \frac{1}{5} \right)^{2} \bullet \left( \frac{1}{5} \right)^{15} =$$

  $$\left( - \frac{9}{7} \right)^{m} \bullet \left( - \frac{9}{7} \right)^{n} =$$   $$\frac{ab^{3}}{b^{2}} =$$
  ----------------------------------------------------------------------------------------------------------------------------------------------------------------

3.  Let the dimensions of a rectangle be
    $\left( 4 \times (871209)^{5} + \ 3 \times 49762105 \right)\ ft.$ by
    $\left( 7 \times (871209)^{3} - (49762105)^{4} \right)\ ft.$
    Determine the area of the rectangle. (Hint: You do not need to
    expand all the powers.)

4.  A rectangular area of land is being sold off in smaller pieces. The
    total area of the land is $2^{15}$ square miles. The pieces being
    sold are $8^{3}$ square miles in size. How many smaller pieces of
    land can be sold at the stated size? Compute the actual number of
    pieces.
