Lesson 4: Numbers Raised to the Zeroth Power

Classwork

We have shown that for any numbers $x$, $y$, and any positive integers
$m$, $n$, the following holds

$x^{m} \bullet x^{n} = x^{m + n}$ (1)

$\left( x^{m} \right)^{n} = x^{mn}$ (2)

$(xy)^{n} = x^{n}y^{n}$. (3)

**Definition:**
\_\_\_\_\_\_\_\_\_\_\_\_\_\_\_\_\_\_\_\_\_\_\_\_\_\_\_\_\_\_\_\_\_\_\_\_\_\_\_\_\_\_\_\_\_\_\_\_\_\_\_\_\_\_\_\_\_\_\_\_\_\_\_\_\_\_\_\_\_\_\_\_\_\_\_

Exercise 1

List all possible cases of whole numbers $m$ and $n$ for identity (1).
More precisely, when $m > 0$ and $n > 0$, we already know that (1) is
correct. What are the other possible cases of $m\ $and $n$ for which (1)
is yet to be verified?

Exercise 2

Check that equation (1) is correct for each of the cases listed in
Exercise 1.

Exercise 3

Do the same with equation (2) by checking it case-by-case.

Exercise 4

Do the same with equation (3) by checking it case-by-case.

Exercise 5

Write the expanded form of $8,374\ $using exponential notation.

**Exercise 6**

Write the expanded form of $6,985,062\ $using exponential notation.

Problem Set

Let $x,\ y$ be numbers $(x,\ y \neq 0)$. Simplify each of the following
expressions.

+---------------------------------------------------------+---------------------------------------------------------------------------------------------------------------------------+
| $$\frac{y^{12}}{y^{12}} =$$                             | $$9^{15} \bullet \frac{1}{9^{15}} =$$                                                                                     |
+=========================================================+===========================================================================================================================+
| $$\left( 7(123456.789)^{4} \right)^{0} =$$              | $$2^{2} \bullet \frac{1}{2^{5}} \bullet 2^{5} \bullet \frac{1}{2^{2}} = \frac{2^{2}}{2^{2}} \bullet \frac{2^{5}}{2^{5}}$$ |
+---------------------------------------------------------+---------------------------------------------------------------------------------------------------------------------------+
| $$\frac{x^{41}}{y^{15}} \bullet \frac{y^{15}}{x^{41}} = \frac{x^{41} \bullet y^{15}}{y^{15} \bullet x^{41}}$$                                                                       |
+-------------------------------------------------------------------------------------------------------------------------------------------------------------------------------------+
